Finalizing `eku` and trying to use it (#43).

src/riot/x509/X509.ExtFields.ExtendedKeyUsage.fst
@@ -26,9 +26,13 @@ let valid_keyPurposeIDs
 : Type0
 = 0 < List.length oids /\ (List.length oids) < 10
 
+let keyPurposeIDs_oids_t
+: Type
+= oids: list (datatype_of_asn1_type OID) { valid_keyPurposeIDs oids }
+
 noextract inline_for_extraction
 let rec x509_keyPurposeIDs_t
-  (oids: list (datatype_of_asn1_type OID) { valid_keyPurposeIDs oids})
+  (oids: keyPurposeIDs_oids_t)
 : Tot (Type0)
   (decreases (List.length oids))
 = let oids', oid = List.Tot.Base.unsnoc oids in
@@ -39,9 +43,31 @@ let rec x509_keyPurposeIDs_t
             `tuple2`
             get_parser_type (parse_asn1_oid_TLV_of oid) )
 
+let lemma_x509_keyPurposeIDs_unique
+  (oids: keyPurposeIDs_oids_t)
+: Lemma
+  (ensures forall (x1: x509_keyPurposeIDs_t oids)
+             (x2: x509_keyPurposeIDs_t oids).
+               x1 == x2 )
+= let rec lemma_x509_keyPurposeIDs_unique_prf
+    (oids: keyPurposeIDs_oids_t)
+    (x1 x2: x509_keyPurposeIDs_t oids)
+  : Lemma
+    (ensures x1 == x2 )
+    (decreases (List.length oids))
+  = let oids', oid = List.Tot.Base.unsnoc oids in
+    List.Tot.Properties.lemma_unsnoc_length oids;
+    match oids' with
+    | [] -> ( () )
+    | _  -> ( let x1 = x1 <: x509_keyPurposeIDs_t oids' `tuple2` get_parser_type (parse_asn1_oid_TLV_of oid) in
+              let x2 = x2 <: x509_keyPurposeIDs_t oids' `tuple2` get_parser_type (parse_asn1_oid_TLV_of oid) in
+              assert ( snd x1 == snd x2 );
+              lemma_x509_keyPurposeIDs_unique_prf oids' (fst x1) (fst x2) ) in
+  Classical.forall_intro_2 (lemma_x509_keyPurposeIDs_unique_prf oids)
+
 noextract inline_for_extraction
 let rec get_x509_keyPurposeIDs
-  (oids: list (datatype_of_asn1_type OID) { valid_keyPurposeIDs oids})
+  (oids: keyPurposeIDs_oids_t)
 : Tot (x509_keyPurposeIDs_t oids)
   (decreases (List.length oids))
 = let oids', oid = List.Tot.Base.unsnoc oids in
@@ -54,7 +80,7 @@ let rec get_x509_keyPurposeIDs
                 get_parser_type (parse_asn1_oid_TLV_of oid) )
 
 let rec parse_x509_keyPurposeIDs_kind
-  (oids: list (datatype_of_asn1_type OID) { valid_keyPurposeIDs oids})
+  (oids: keyPurposeIDs_oids_t)
 : Tot (k: parser_kind { Mkparser_kind'?.parser_kind_subkind k == Some ParserStrong })
   (decreases (List.length oids))
 = let oids', oid = List.Tot.Base.unsnoc oids in
@@ -66,7 +92,7 @@ let rec parse_x509_keyPurposeIDs_kind
             get_parser_kind (parse_asn1_oid_TLV_of oid) )
 
 let rec parse_x509_keyPurposeIDs
-  (oids: list (datatype_of_asn1_type OID) {valid_keyPurposeIDs oids})
+  (oids: keyPurposeIDs_oids_t)
 : Tot (parser (parse_x509_keyPurposeIDs_kind oids) (x509_keyPurposeIDs_t oids))
   (decreases (List.length oids))
 = let oids', oid = List.Tot.Base.unsnoc oids in
@@ -78,7 +104,7 @@ let rec parse_x509_keyPurposeIDs
             parse_asn1_oid_TLV_of oid )
 
 let rec serialize_x509_keyPurposeIDs
-  (oids: list (datatype_of_asn1_type OID) {valid_keyPurposeIDs oids})
+  (oids: keyPurposeIDs_oids_t)
 : Tot (serializer (parse_x509_keyPurposeIDs oids))
   (decreases (List.length oids))
 = let oids', oid = List.Tot.Base.unsnoc oids in
@@ -91,7 +117,7 @@ let rec serialize_x509_keyPurposeIDs
 
 noextract
 let rec serialize32_x509_keyPurposeIDs_backwards
-  (oids: list (datatype_of_asn1_type OID) {valid_keyPurposeIDs oids})
+  (oids: keyPurposeIDs_oids_t)
 : Tot (serializer32_backwards (serialize_x509_keyPurposeIDs oids))
   (decreases (List.length oids))
 = let oids', oid = List.Tot.Base.unsnoc oids in
@@ -102,143 +128,140 @@ let rec serialize32_x509_keyPurposeIDs_backwards
             `serialize32_nondep_then_backwards`
             serialize32_asn1_oid_TLV_of_backwards oid )
 
-// noextract
-// let postprocess_listops ()
-// : T.Tac unit
-// = T.norm [delta_only [
-//   `%FStar.List.Tot.Base.unsnoc;
-//   `%FStar.List.Tot.Base.splitAt;
-//   `%FStar.List.Tot.Base.length;
-//   `%FStar.List.Tot.Base.hd;
-//   ]; primops; zeta; iota]; T.trefl ()
-
 // [@@T.postprocess_with postprocess_listops]
 let rec serialize_x509_keyPurposeIDs_unfold_spec
-  (oids: list (datatype_of_asn1_type OID) {valid_keyPurposeIDs oids})
-  (x: x509_keyPurposeIDs_t oids)
+  (oids: keyPurposeIDs_oids_t)
+  // (x: x509_keyPurposeIDs_t oids)
 : GTot (_)
   (decreases (List.length oids))
-= let oids', oid = List.Tot.Base.unsnoc oids in
+= let x = get_x509_keyPurposeIDs oids in
+  let oids', oid = List.Tot.Base.unsnoc oids in
   List.Tot.Properties.lemma_unsnoc_length oids;
   match oids' with
   | [] -> ( serialize (serialize_asn1_oid_TLV_of oid) x )
   | _  -> ( let x = x <: x509_keyPurposeIDs_t oids' `tuple2` get_parser_type (parse_asn1_oid_TLV_of oid) in
-            serialize_x509_keyPurposeIDs_unfold_spec oids' (fst x)
+            serialize_x509_keyPurposeIDs_unfold_spec oids'
             `Seq.append`
             serialize (serialize_asn1_oid_TLV_of oid) (snd x) )
 
 // [@@T.postprocess_with postprocess_listops]
 let rec lemma_serialize_x509_keyPurposeIDs_unfold
-  (oids: list (datatype_of_asn1_type OID) {valid_keyPurposeIDs oids})
-  (x: x509_keyPurposeIDs_t oids)
+  (oids: keyPurposeIDs_oids_t)
+  // (x: x509_keyPurposeIDs_t oids)
 : Lemma (ensures
-  serialize (serialize_x509_keyPurposeIDs oids) x ==
-  serialize_x509_keyPurposeIDs_unfold_spec oids x
+  serialize (serialize_x509_keyPurposeIDs oids) (get_x509_keyPurposeIDs oids) ==
+  serialize_x509_keyPurposeIDs_unfold_spec oids
 )
   (decreases (List.length oids))
 = let oids', oid = List.Tot.Base.unsnoc oids in
   List.Tot.Properties.lemma_unsnoc_length oids;
   match oids' with
   | [] -> ()
-  | _  -> ( let x = x <: x509_keyPurposeIDs_t oids' `tuple2` get_parser_type (parse_asn1_oid_TLV_of oid) in
+  | _  -> ( let x = (get_x509_keyPurposeIDs oids)
+                     <: x509_keyPurposeIDs_t oids' `tuple2`
+                        get_parser_type (parse_asn1_oid_TLV_of oid) in
             serialize_nondep_then_eq
             (* s1 *) (serialize_x509_keyPurposeIDs oids')
             (* s2 *) (serialize_asn1_oid_TLV_of oid)
             (* in *) x;
-            lemma_serialize_x509_keyPurposeIDs_unfold oids' (fst x) )
+            lemma_serialize_x509_keyPurposeIDs_unfold oids' )
 
 (*
  * Reveals the structure and size of all oids
- * Use with `lemma_serialize_x509_keyPurposeIDs_size_norm` (defined later)
+ * Use with fuels or `lemma_serialize_x509_keyPurposeIDs_size_norm` (defined later)
  *)
 
 let rec predicate_serialize_x509_keyPurposeIDs_size_oids
-  (oids: list (datatype_of_asn1_type OID) {valid_keyPurposeIDs oids})
-  (x: x509_keyPurposeIDs_t oids)
+  (oids: keyPurposeIDs_oids_t)
+  // (x: x509_keyPurposeIDs_t oids)
 : GTot (Type0)
   (decreases (List.length oids))
-= lemma_serialize_x509_keyPurposeIDs_unfold oids x;
+= lemma_serialize_x509_keyPurposeIDs_unfold oids;
   let oids', oid = List.Tot.Base.unsnoc oids in
   List.Tot.Properties.lemma_unsnoc_length oids;
   match oids' with
-  | [] -> ( length_of_opaque_serialization (serialize_asn1_oid_TLV_of x) x ==
-            length_of_TLV OID (length_of_oid x) )
-  | _  -> ( let x = x <: x509_keyPurposeIDs_t oids' `tuple2` get_parser_type (parse_asn1_oid_TLV_of oid) in
+  | [] -> ( length_of_opaque_serialization (serialize_asn1_oid_TLV_of (get_x509_keyPurposeIDs oids)) (get_x509_keyPurposeIDs oids) ==
+            length_of_TLV OID (length_of_oid (get_x509_keyPurposeIDs oids)) )
+  | _  -> ( let x = (get_x509_keyPurposeIDs oids) <: x509_keyPurposeIDs_t oids' `tuple2` get_parser_type (parse_asn1_oid_TLV_of oid) in
             length_of_opaque_serialization (serialize_asn1_oid_TLV_of (snd x)) (snd x) ==
             length_of_TLV OID (length_of_oid (snd x)) /\
-            predicate_serialize_x509_keyPurposeIDs_size_oids oids' (fst x) )
+            predicate_serialize_x509_keyPurposeIDs_size_oids oids' )
 
 let rec serialize_x509_keyPurposeIDs_size_spec
-  (oids: list (datatype_of_asn1_type OID) {valid_keyPurposeIDs oids})
-  (x: x509_keyPurposeIDs_t oids)
+  (oids: keyPurposeIDs_oids_t)
+  // (x: x509_keyPurposeIDs_t oids)
 : GTot (nat)
   (decreases (List.length oids))
 = let oids', oid = List.Tot.Base.unsnoc oids in
   List.Tot.Properties.lemma_unsnoc_length oids;
   match oids' with
-  | [] -> ( length_of_opaque_serialization (serialize_asn1_oid_TLV_of oid) x )
-  | _  -> ( let x = x <: x509_keyPurposeIDs_t oids' `tuple2` get_parser_type (parse_asn1_oid_TLV_of oid) in
-            serialize_x509_keyPurposeIDs_size_spec oids' (fst x) +
+  | [] -> ( length_of_opaque_serialization (serialize_asn1_oid_TLV_of oid) (get_x509_keyPurposeIDs oids) )
+  | _  -> ( let x = (get_x509_keyPurposeIDs oids) <: x509_keyPurposeIDs_t oids' `tuple2` get_parser_type (parse_asn1_oid_TLV_of oid) in
+            serialize_x509_keyPurposeIDs_size_spec oids' +
             length_of_opaque_serialization (serialize_asn1_oid_TLV_of (snd x)) (snd x) )
-            // Seq.length (serialize (serialize_asn1_oid_TLV_of oid) (snd x)) )
 
 let rec lemma_serialize_x509_keyPurposeIDs_size
-  (oids: list (datatype_of_asn1_type OID) {valid_keyPurposeIDs oids})
-  (x: x509_keyPurposeIDs_t oids)
+  (oids: keyPurposeIDs_oids_t)
+  // (x: x509_keyPurposeIDs_t oids)
 : Lemma (ensures
-  length_of_opaque_serialization (serialize_x509_keyPurposeIDs oids) x ==
-  serialize_x509_keyPurposeIDs_size_spec oids x /\
-  predicate_serialize_x509_keyPurposeIDs_size_oids oids x
+  length_of_opaque_serialization (serialize_x509_keyPurposeIDs oids) (get_x509_keyPurposeIDs oids) ==
+  serialize_x509_keyPurposeIDs_size_spec oids /\
+  predicate_serialize_x509_keyPurposeIDs_size_oids oids
 )
   (decreases (List.length oids))
-= lemma_serialize_x509_keyPurposeIDs_unfold oids x;
+= lemma_serialize_x509_keyPurposeIDs_unfold oids;
   let oids', oid = List.Tot.Base.unsnoc oids in
   List.Tot.Properties.lemma_unsnoc_length oids;
   match oids' with
-  | [] -> ( lemma_serialize_asn1_oid_TLV_of_size x x )
-  | _  -> ( let x = x <: x509_keyPurposeIDs_t oids' `tuple2` get_parser_type (parse_asn1_oid_TLV_of oid) in
+  | [] -> ( lemma_serialize_asn1_oid_TLV_of_size (get_x509_keyPurposeIDs oids) (get_x509_keyPurposeIDs oids) )
+  | _  -> ( let x = (get_x509_keyPurposeIDs oids) <: x509_keyPurposeIDs_t oids' `tuple2` get_parser_type (parse_asn1_oid_TLV_of oid) in
             lemma_serialize_asn1_oid_TLV_of_size (snd x) (snd x);
-            lemma_serialize_x509_keyPurposeIDs_unfold oids' (fst x);
-            lemma_serialize_x509_keyPurposeIDs_size oids' (fst x) )
+            lemma_serialize_x509_keyPurposeIDs_unfold oids';
+            lemma_serialize_x509_keyPurposeIDs_size   oids' )
+
+let valid_x509_ext_keyPurposeIDs_ingredients
+  (oids: keyPurposeIDs_oids_t)
+  // (x: x509_keyPurposeIDs_t oids)
+: Type0
+= serialize_x509_keyPurposeIDs_size_spec oids // (get_x509_keyPurposeIDs oids)
+  <= asn1_value_length_max_of_type SEQUENCE
 
 let rec length_of_x509_keyPurposeIDs
-  (oids: list (datatype_of_asn1_type OID) {valid_keyPurposeIDs oids})
-  (x: x509_keyPurposeIDs_t oids
-      { serialize_x509_keyPurposeIDs_size_spec oids x
-        <= asn1_value_length_max_of_type SEQUENCE })
+  (oids: keyPurposeIDs_oids_t
+         { valid_x509_ext_keyPurposeIDs_ingredients oids })
+  // (x: x509_keyPurposeIDs_t oids
+  //     { valid_x509_ext_keyPurposeIDs_ingredients oids x })
 : GTot (l: asn1_value_length_of_type SEQUENCE
-           { l == serialize_x509_keyPurposeIDs_size_spec oids x })
+           { l == serialize_x509_keyPurposeIDs_size_spec oids })
   (decreases (List.length oids))
 = let oids', oid = List.Tot.Base.unsnoc oids in
   List.Tot.Properties.lemma_unsnoc_length oids;
-  lemma_serialize_x509_keyPurposeIDs_size oids x;
+  lemma_serialize_x509_keyPurposeIDs_size oids;
   match oids' with
-  | [] -> ( length_of_asn1_primitive_TLV #OID x )
-  | _  -> ( let x = x <: x509_keyPurposeIDs_t oids' `tuple2` get_parser_type (parse_asn1_oid_TLV_of oid) in
-            lemma_serialize_x509_keyPurposeIDs_size oids' (fst x);
-            length_of_x509_keyPurposeIDs oids' (fst x) +
+  | [] -> ( length_of_asn1_primitive_TLV #OID (get_x509_keyPurposeIDs oids) )
+  | _  -> ( let x = (get_x509_keyPurposeIDs oids) <: x509_keyPurposeIDs_t oids' `tuple2` get_parser_type (parse_asn1_oid_TLV_of oid) in
+            lemma_serialize_x509_keyPurposeIDs_size oids';
+            length_of_x509_keyPurposeIDs oids' +
             length_of_asn1_primitive_TLV #OID (snd x) )
 
 noextract
 let rec len_of_x509_keyPurposeIDs
-  (oids: list (datatype_of_asn1_type OID) {valid_keyPurposeIDs oids})
-  (x: x509_keyPurposeIDs_t oids
-      { serialize_x509_keyPurposeIDs_size_spec oids x
-        <= asn1_value_length_max_of_type SEQUENCE })
+  (oids: keyPurposeIDs_oids_t
+         { valid_x509_ext_keyPurposeIDs_ingredients oids })
+  // (x: x509_keyPurposeIDs_t oids
+  //     { valid_x509_ext_keyPurposeIDs_ingredients oids x })
 : Tot (len: asn1_value_int32_of_type SEQUENCE
-           { v len == serialize_x509_keyPurposeIDs_size_spec oids x })
+           { v len == length_of_x509_keyPurposeIDs oids })
   (decreases (List.length oids))
 = let oids', oid = List.Tot.Base.unsnoc oids in
   List.Tot.Properties.lemma_unsnoc_length oids;
-  lemma_serialize_x509_keyPurposeIDs_size oids x;
+  lemma_serialize_x509_keyPurposeIDs_size oids;
   match oids' with
-  | [] -> ( len_of_asn1_primitive_TLV #OID x )
-  | _  -> ( let x = x <: x509_keyPurposeIDs_t oids' `tuple2` get_parser_type (parse_asn1_oid_TLV_of oid) in
-            lemma_serialize_x509_keyPurposeIDs_size oids' (fst x);
-            len_of_x509_keyPurposeIDs oids' (fst x) +
+  | [] -> ( len_of_asn1_primitive_TLV #OID (get_x509_keyPurposeIDs oids) )
+  | _  -> ( let x = (get_x509_keyPurposeIDs oids) <: x509_keyPurposeIDs_t oids' `tuple2` get_parser_type (parse_asn1_oid_TLV_of oid) in
+            lemma_serialize_x509_keyPurposeIDs_size oids';
+            len_of_x509_keyPurposeIDs oids' +
             len_of_asn1_primitive_TLV #OID (snd x) )
-
-#set-options "--fuel 0 --ifuel 0"
 
 (*
  * Payload
@@ -248,12 +271,12 @@ open X509.BasicFields.Extension2
 
 unfold inline_for_extraction
 let x509_ext_key_usage_payload_t
-  (oids: list (datatype_of_asn1_type OID) {valid_keyPurposeIDs oids})
+  (oids: keyPurposeIDs_oids_t)
 = inbound_sequence_value_of
   (**) (serialize_x509_keyPurposeIDs oids)
 
 let parse_x509_ext_key_usage_payload
-  (oids: list (datatype_of_asn1_type OID) {valid_keyPurposeIDs oids})
+  (oids: keyPurposeIDs_oids_t)
 : parser _ (x509_ext_key_usage_payload_t oids)
 = x509_ext_key_usage_payload_t oids
   `coerce_parser`
@@ -261,7 +284,7 @@ let parse_x509_ext_key_usage_payload
   (**) (serialize_x509_keyPurposeIDs oids)
 
 let serialize_x509_ext_key_usage_payload
-  (oids: list (datatype_of_asn1_type OID) {valid_keyPurposeIDs oids})
+  (oids: keyPurposeIDs_oids_t)
 : serializer (parse_x509_ext_key_usage_payload oids)
 = coerce_parser_serializer
     (_)
@@ -271,102 +294,102 @@ let serialize_x509_ext_key_usage_payload
 
 noextract inline_for_extraction
 let serialize32_x509_ext_key_usage_payload_backwards
-  (oids: list (datatype_of_asn1_type OID) {valid_keyPurposeIDs oids})
-  (s32: serializer32_backwards (serialize_x509_keyPurposeIDs oids))
+  (oids: keyPurposeIDs_oids_t)
 : serializer32_backwards (serialize_x509_ext_key_usage_payload oids)
 = coerce_serializer32_backwards
     (_)
     (serialize32_asn1_sequence_TLV_backwards
-    (**) (s32))
+    (**) (serialize32_x509_keyPurposeIDs_backwards oids))
     ()
 
 let lemma_serialize_x509_ext_key_usage_payload_unfold
-  (oids: list (datatype_of_asn1_type OID) {valid_keyPurposeIDs oids})
-  (x: x509_ext_key_usage_payload_t oids)
+  (oids: keyPurposeIDs_oids_t
+         { valid_x509_ext_keyPurposeIDs_ingredients oids })
+  // (x: x509_ext_key_usage_payload_t oids)
 : Lemma (
+  lemma_serialize_x509_keyPurposeIDs_size oids;
   predicate_serialize_asn1_sequence_TLV_unfold
   (**) (serialize_x509_keyPurposeIDs oids)
-  (**) (x)
+  (**) (get_x509_keyPurposeIDs oids)
 )
-= lemma_serialize_asn1_sequence_TLV_unfold
+= lemma_serialize_x509_keyPurposeIDs_size oids;
+  lemma_serialize_asn1_sequence_TLV_unfold
   (**) (serialize_x509_keyPurposeIDs oids)
-  (**) (x)
+  (**) (get_x509_keyPurposeIDs oids)
 
 let lemma_serialize_x509_ext_key_usage_payload_size
-  (oids: list (datatype_of_asn1_type OID) {valid_keyPurposeIDs oids})
-  (x: x509_ext_key_usage_payload_t oids)
+  (oids: keyPurposeIDs_oids_t
+         { valid_x509_ext_keyPurposeIDs_ingredients oids })
+  // (x: x509_ext_key_usage_payload_t oids)
 : Lemma (
+  lemma_serialize_x509_keyPurposeIDs_size oids;
   predicate_serialize_asn1_sequence_TLV_size
   (**) (serialize_x509_keyPurposeIDs oids)
-  (**) (x)
+  (**) (get_x509_keyPurposeIDs oids)
 )
-= lemma_serialize_asn1_sequence_TLV_size
+= lemma_serialize_x509_keyPurposeIDs_size oids;
+  lemma_serialize_asn1_sequence_TLV_size
   (**) (serialize_x509_keyPurposeIDs oids)
-  (**) (x)
+  (**) (get_x509_keyPurposeIDs oids)
 
-let length_of_x509_ext_key_usage_payload_unbound
-  (oids: list (datatype_of_asn1_type OID) {valid_keyPurposeIDs oids})
-  (x: x509_keyPurposeIDs_t oids
-      { serialize_x509_keyPurposeIDs_size_spec oids x
-        <= asn1_value_length_max_of_type SEQUENCE })
+let length_of_x509_ext_key_usage_payload_unbounded
+  (oids: keyPurposeIDs_oids_t
+         { valid_x509_ext_keyPurposeIDs_ingredients oids })
 : GTot (asn1_TLV_length_of_type SEQUENCE)
 = length_of_TLV
     (SEQUENCE)
-    (length_of_x509_keyPurposeIDs oids x)
+    (length_of_x509_keyPurposeIDs oids)
+
+let valid_x509_ext_key_usage_payload_ingredients
+  (oids: keyPurposeIDs_oids_t)
+= valid_x509_ext_keyPurposeIDs_ingredients oids /\
+  length_of_x509_ext_key_usage_payload_unbounded oids
+  <= asn1_value_length_max_of_type OCTET_STRING
 
 let length_of_x509_ext_key_usage_payload
-  (oids: list (datatype_of_asn1_type OID) {valid_keyPurposeIDs oids})
-  (x: x509_keyPurposeIDs_t oids
-      { serialize_x509_keyPurposeIDs_size_spec oids x
-        <= asn1_value_length_max_of_type SEQUENCE /\
-        length_of_x509_ext_key_usage_payload_unbound oids x
-        <= asn1_value_length_max_of_type OCTET_STRING })
-: GTot (asn1_value_length_of_type OCTET_STRING)
+  (oids: keyPurposeIDs_oids_t
+      { valid_x509_ext_key_usage_payload_ingredients oids })
+: GTot (l: asn1_value_length_of_type OCTET_STRING
+           { l == length_of_x509_ext_key_usage_payload_unbounded oids })
 = length_of_TLV
     (SEQUENCE)
-    (length_of_x509_keyPurposeIDs oids x)
+    (length_of_x509_keyPurposeIDs oids)
 
 noextract inline_for_extraction
 let len_of_x509_ext_key_usage_payload
-  (oids: list (datatype_of_asn1_type OID) {valid_keyPurposeIDs oids})
-  (x: x509_keyPurposeIDs_t oids
-      { serialize_x509_keyPurposeIDs_size_spec oids x
-        <= asn1_value_length_max_of_type SEQUENCE /\
-        length_of_x509_ext_key_usage_payload_unbound oids x
-        <= asn1_value_length_max_of_type OCTET_STRING })
+  (oids: keyPurposeIDs_oids_t
+      { valid_x509_ext_key_usage_payload_ingredients oids })
 : Tot (len: asn1_value_int32_of_type OCTET_STRING
-            { v len == length_of_x509_ext_key_usage_payload oids x })
+            { v len == length_of_x509_ext_key_usage_payload oids })
 = len_of_TLV
     (SEQUENCE)
-    (len_of_x509_keyPurposeIDs oids x)
+    (len_of_x509_keyPurposeIDs oids)
 
 let lemma_serialize_x509_ext_key_usage_payload_size_exact
-  (oids: list (datatype_of_asn1_type OID) {valid_keyPurposeIDs oids})
-  (x: x509_ext_key_usage_payload_t oids
-      { serialize_x509_keyPurposeIDs_size_spec oids x
-        <= asn1_value_length_max_of_type SEQUENCE /\
-        length_of_x509_ext_key_usage_payload_unbound oids x
-        <= asn1_value_length_max_of_type OCTET_STRING })
+  (oids: keyPurposeIDs_oids_t
+         { valid_x509_ext_key_usage_payload_ingredients oids })
+  // (x: x509_ext_key_usage_payload_t oids)
 : Lemma (
-  length_of_opaque_serialization (serialize_x509_ext_key_usage_payload oids) x ==
-  length_of_x509_ext_key_usage_payload oids x
+  lemma_serialize_x509_keyPurposeIDs_size oids;
+  length_of_opaque_serialization (serialize_x509_ext_key_usage_payload oids) (get_x509_keyPurposeIDs oids) ==
+  length_of_x509_ext_key_usage_payload oids
 )
-= lemma_serialize_x509_ext_key_usage_payload_unfold oids x;
-  lemma_serialize_x509_ext_key_usage_payload_size oids x;
-    lemma_serialize_x509_keyPurposeIDs_size oids x
+= lemma_serialize_x509_ext_key_usage_payload_unfold oids;
+  lemma_serialize_x509_ext_key_usage_payload_size oids;
+    lemma_serialize_x509_keyPurposeIDs_size oids
 
 (*
  * Main
  *)
 
 let x509_ext_key_usage_t
-  (oids: list (datatype_of_asn1_type OID) {valid_keyPurposeIDs oids})
+  (oids: keyPurposeIDs_oids_t)
 = x509_extension_t
   (**) (OID_EXTENDED_KEY_USAGE)
   (**) (serialize_x509_ext_key_usage_payload oids)
 
 let parse_x509_ext_key_usage
-  (oids: list (datatype_of_asn1_type OID) {valid_keyPurposeIDs oids})
+  (oids: keyPurposeIDs_oids_t)
 : parser parse_x509_extension_kind (x509_ext_key_usage_t oids)
 = x509_ext_key_usage_t oids
   `coerce_parser`
@@ -375,7 +398,7 @@ let parse_x509_ext_key_usage
   (**) (serialize_x509_ext_key_usage_payload oids)
 
 let serialize_x509_ext_key_usage
-  (oids: list (datatype_of_asn1_type OID) {valid_keyPurposeIDs oids})
+  (oids: keyPurposeIDs_oids_t)
 : serializer (parse_x509_ext_key_usage oids)
 = coerce_parser_serializer
     (parse_x509_ext_key_usage oids)
@@ -386,30 +409,32 @@ let serialize_x509_ext_key_usage
 
 noextract inline_for_extraction
 let serialize32_x509_ext_key_usage_backwards
-  (oids: list (datatype_of_asn1_type OID) {valid_keyPurposeIDs oids})
-  (s32: serializer32_backwards (serialize_x509_keyPurposeIDs oids))
+  (oids: keyPurposeIDs_oids_t)
 : serializer32_backwards (serialize_x509_ext_key_usage oids)
 = coerce_serializer32_backwards
     (_)
     (serialize32_x509_extension_backwards
     (**) (OID_EXTENDED_KEY_USAGE)
-    (**) (serialize32_x509_ext_key_usage_payload_backwards oids s32))
+    (**) (serialize32_x509_ext_key_usage_payload_backwards oids))
     ()
 
 let lemma_serialize_x509_ext_key_usage_unfold
-  (oids: list (datatype_of_asn1_type OID) {valid_keyPurposeIDs oids})
+  (oids: keyPurposeIDs_oids_t
+         { valid_x509_ext_key_usage_payload_ingredients oids })
   (x: x509_ext_key_usage_t oids)
-: Lemma ( predicate_serialize_x509_extension_unfold
+: Lemma ( lemma_serialize_x509_ext_key_usage_payload_size_exact oids;
+          predicate_serialize_x509_extension_unfold
           (**) (OID_EXTENDED_KEY_USAGE)
           (**) (serialize_x509_ext_key_usage_payload oids)
           (**) (x) )
-= lemma_serialize_x509_extension_unfold
+= lemma_serialize_x509_ext_key_usage_payload_size_exact oids;
+  lemma_serialize_x509_extension_unfold
   (**) (OID_EXTENDED_KEY_USAGE)
   (**) (serialize_x509_ext_key_usage_payload oids)
   (**) (x)
 
 let lemma_serialize_x509_ext_key_usage_size
-  (oids: list (datatype_of_asn1_type OID) {valid_keyPurposeIDs oids})
+  (oids: keyPurposeIDs_oids_t)
   (x: x509_ext_key_usage_t oids)
 : Lemma ( predicate_serialize_x509_extension_size
           (**) (OID_EXTENDED_KEY_USAGE)
@@ -420,121 +445,117 @@ let lemma_serialize_x509_ext_key_usage_size
   (**) (serialize_x509_ext_key_usage_payload oids)
   (**) (x)
 
+let valid_x509_ext_key_usage_ingredients
+  (oids: keyPurposeIDs_oids_t)
+  // (kps: x509_keyPurposeIDs_t oids)
+: Type0
+= valid_x509_ext_key_usage_payload_ingredients oids /\
+ (let _ = lemma_serialize_x509_keyPurposeIDs_size oids;
+          lemma_serialize_x509_ext_key_usage_payload_size_exact oids in
+  length_of_x509_extension_payload_unbounded
+    (OID_EXTENDED_KEY_USAGE)
+    (serialize_x509_ext_key_usage_payload oids)
+    (get_x509_keyPurposeIDs oids <: x509_ext_key_usage_payload_t oids)
+    (length_of_x509_ext_key_usage_payload oids)
+  <= asn1_value_length_max_of_type (SEQUENCE))
+
 let length_of_x509_ext_key_usage
-  (oids: list (datatype_of_asn1_type OID) {valid_keyPurposeIDs oids})
-  (x: x509_keyPurposeIDs_t oids
-      { serialize_x509_keyPurposeIDs_size_spec oids x
-        <= asn1_value_length_max_of_type SEQUENCE /\
-        length_of_x509_ext_key_usage_payload_unbound oids x
-        <= asn1_value_length_max_of_type OCTET_STRING /\
-       (let _ = lemma_serialize_x509_keyPurposeIDs_size oids x;
-                lemma_serialize_x509_ext_key_usage_payload_size_exact oids x in
-        length_of_x509_extension_payload_unbounded
-          (OID_EXTENDED_KEY_USAGE)
-          (serialize_x509_ext_key_usage_payload oids)
-          (x <: x509_ext_key_usage_payload_t oids)
-          (length_of_x509_ext_key_usage_payload oids x)
-        <= asn1_value_length_max_of_type (SEQUENCE)) })
+  (oids: keyPurposeIDs_oids_t
+         { valid_x509_ext_key_usage_ingredients oids })
+  // (kps: x509_keyPurposeIDs_t oids
+  //       { valid_x509_ext_key_usage_ingredients oids kps })
 : GTot (asn1_TLV_length_of_type SEQUENCE)
-= lemma_serialize_x509_keyPurposeIDs_size oids x;
-  lemma_serialize_x509_ext_key_usage_payload_size_exact oids x;
+= lemma_serialize_x509_keyPurposeIDs_size oids;
+  lemma_serialize_x509_ext_key_usage_payload_size_exact oids;
   length_of_x509_extension
     (OID_EXTENDED_KEY_USAGE)
     (serialize_x509_ext_key_usage_payload oids)
-    (x <: x509_ext_key_usage_payload_t oids)
-    (length_of_x509_ext_key_usage_payload oids x)
+    ((get_x509_keyPurposeIDs oids) <: x509_ext_key_usage_payload_t oids)
+    (length_of_x509_ext_key_usage_payload oids)
 
 let len_of_x509_ext_key_usage
-  (oids: list (datatype_of_asn1_type OID) {valid_keyPurposeIDs oids})
-  (x: x509_keyPurposeIDs_t oids
-      { serialize_x509_keyPurposeIDs_size_spec oids x
-        <= asn1_value_length_max_of_type SEQUENCE /\
-        length_of_x509_ext_key_usage_payload_unbound oids x
-        <= asn1_value_length_max_of_type OCTET_STRING /\
-       (let _ = lemma_serialize_x509_keyPurposeIDs_size oids x;
-                lemma_serialize_x509_ext_key_usage_payload_size_exact oids x in
-        length_of_x509_extension_payload_unbounded
-          (OID_EXTENDED_KEY_USAGE)
-          (serialize_x509_ext_key_usage_payload oids)
-          (x <: x509_ext_key_usage_payload_t oids)
-          (length_of_x509_ext_key_usage_payload oids x)
-        <= asn1_value_length_max_of_type (SEQUENCE)) })
+  (oids: keyPurposeIDs_oids_t
+         { valid_x509_ext_key_usage_ingredients oids })
+  // (kps: x509_keyPurposeIDs_t oids
+  //       { valid_x509_ext_key_usage_ingredients oids kps })
 : Tot (len: asn1_TLV_int32_of_type SEQUENCE
-            { v len == length_of_x509_ext_key_usage oids x })
-= lemma_serialize_x509_keyPurposeIDs_size oids x;
-  lemma_serialize_x509_ext_key_usage_payload_size_exact oids x;
+            { v len == length_of_x509_ext_key_usage oids })
+= lemma_serialize_x509_keyPurposeIDs_size oids;
+  lemma_serialize_x509_ext_key_usage_payload_size_exact oids;
   len_of_x509_extension
     (OID_EXTENDED_KEY_USAGE)
     (serialize_x509_ext_key_usage_payload oids)
-    (x <: x509_ext_key_usage_payload_t oids)
-    (len_of_x509_ext_key_usage_payload oids x)
+    (get_x509_keyPurposeIDs oids <: x509_ext_key_usage_payload_t oids)
+    (len_of_x509_ext_key_usage_payload oids)
 
 let lemma_serialize_x509_ext_key_usage_size_exact
-  (oids: list (datatype_of_asn1_type OID) {valid_keyPurposeIDs oids})
-  (x: x509_ext_key_usage_t oids
-      { serialize_x509_keyPurposeIDs_size_spec oids (snd x)
-        <= asn1_value_length_max_of_type SEQUENCE /\
-        length_of_x509_ext_key_usage_payload_unbound oids (snd x)
-        <= asn1_value_length_max_of_type OCTET_STRING /\
-       (let _ = lemma_serialize_x509_keyPurposeIDs_size oids (snd x);
-                lemma_serialize_x509_ext_key_usage_payload_size_exact oids (snd x) in
-        length_of_x509_extension_payload_unbounded
-          (OID_EXTENDED_KEY_USAGE)
-          (serialize_x509_ext_key_usage_payload oids)
-          ((snd x) <: x509_ext_key_usage_payload_t oids)
-          (length_of_x509_ext_key_usage_payload oids (snd x))
-        <= asn1_value_length_max_of_type (SEQUENCE)) })
+  (oids: keyPurposeIDs_oids_t
+      { valid_x509_ext_key_usage_ingredients oids })
+  (x: x509_ext_key_usage_t oids)
 : Lemma (
   length_of_opaque_serialization (serialize_x509_ext_key_usage oids) x ==
-  length_of_x509_ext_key_usage oids (snd x)
+  length_of_x509_ext_key_usage oids
 )
-= lemma_serialize_x509_ext_key_usage_payload_size_exact oids (snd x);
-  lemma_serialize_x509_keyPurposeIDs_size oids (snd x);
+= lemma_x509_keyPurposeIDs_unique oids;
+  lemma_serialize_x509_ext_key_usage_payload_size_exact oids;
+  lemma_serialize_x509_keyPurposeIDs_size oids;
   lemma_serialize_x509_extension_size_exact
     (OID_EXTENDED_KEY_USAGE)
     (serialize_x509_ext_key_usage_payload oids)
     (x)
-    (length_of_x509_ext_key_usage_payload oids (snd x))
+    (length_of_x509_ext_key_usage_payload oids)
+
+(* TODO: Need to figure out how to easily prove `valid_x509_ext_key_usage_ingredients` *)
 
 #push-options "--z3rlimit 128"
 
 noextract inline_for_extraction
 let x509_get_ext_extendedKeyUsage
-  (oids: list (datatype_of_asn1_type OID) { valid_keyPurposeIDs oids })
+  (oids: keyPurposeIDs_oids_t)
   (criticality: datatype_of_asn1_type BOOLEAN
                 { let kpIDs: x509_keyPurposeIDs_t oids = get_x509_keyPurposeIDs oids in
-                  serialize_x509_keyPurposeIDs_size_spec oids kpIDs
-                  <= asn1_value_length_max_of_type SEQUENCE /\
-                  length_of_x509_ext_key_usage_payload_unbound oids kpIDs
-                  <= asn1_value_length_max_of_type OCTET_STRING /\
-                 (let _ = lemma_serialize_x509_keyPurposeIDs_size oids kpIDs;
-                          lemma_serialize_x509_ext_key_usage_payload_size_exact oids kpIDs in
-                  length_of_x509_extension_payload_unbounded
-                    (OID_EXTENDED_KEY_USAGE)
-                    (serialize_x509_ext_key_usage_payload oids)
-                    (kpIDs)
-                    (length_of_x509_ext_key_usage_payload oids kpIDs)
-                  <= asn1_value_length_max_of_type (SEQUENCE)) })
+                  valid_x509_ext_key_usage_ingredients oids })
 : Tot (x509_ext_key_usage_t oids)
 =
   let kpIDs: x509_keyPurposeIDs_t oids = get_x509_keyPurposeIDs oids in
-  lemma_serialize_x509_keyPurposeIDs_size oids kpIDs;
+  lemma_serialize_x509_keyPurposeIDs_size oids;
 
   let ext_payload: x509_ext_key_usage_payload_t oids = get_x509_keyPurposeIDs oids in
-  lemma_serialize_x509_ext_key_usage_payload_size_exact oids ext_payload;
+  lemma_serialize_x509_ext_key_usage_payload_size_exact oids;
 
   let ext: x509_ext_key_usage_t oids = x509_get_extension
                                          (OID_EXTENDED_KEY_USAGE)
                                          (serialize_x509_ext_key_usage_payload oids)
                                          (ext_payload)
-                                         (len_of_x509_ext_key_usage_payload oids ext_payload)
+                                         (len_of_x509_ext_key_usage_payload oids)
                                          (criticality)
                                          in
 
 (* return *) ext
 
+#push-options "--fuel 4"
 
+// #push-options "--fuel 4"
 
+// noextract unfold inline_for_extraction
+// let oids: keyPurposeIDs_oids_t
+// = [@inline_let] let l = [OID_AT_CN; OID_AT_COUNTRY; OID_AT_ORGANIZATION] in
+//   assert_norm (valid_keyPurposeIDs l);
+//   l
+
+// let ty = x509_keyPurposeIDs_t oids
+
+// let tm: x509_keyPurposeIDs_t oids = get_x509_keyPurposeIDs oids
+
+// let test () =
+//   lemma_serialize_x509_keyPurposeIDs_size oids tm;
+//   // assert (
+//   //   valid_keyPurposeIDs oids /\
+//   //   valid_x509_ext_key_usage_payload_ingredients oids tm /\
+//   //   valid_x509_ext_key_usage_ingredients oids tm
+//   // );
+//   let ext = x509_get_ext_extendedKeyUsage oids true in
+// ()
 
 (* Helpers to unroll recursively defined types and lemmas *)
 
@@ -557,6 +578,8 @@ let norm_steps_x509_keyPurposeIDs
   `%inbound_envelop_tag_with_value_of;
   (* the Low* implementation to extract *)
   `%serialize32_x509_keyPurposeIDs_backwards;
+  `%serialize32_x509_ext_key_usage_payload_backwards;
+  `%serialize32_x509_ext_key_usage_backwards;
   `%serialize_x509_keyPurposeIDs_size_spec;
   `%length_of_x509_keyPurposeIDs;
   `%len_of_x509_keyPurposeIDs;
@@ -596,60 +619,60 @@ let postprocess_x509_keyPurposeIDs
   T.trefl()
 
 let lemma_serialize_x509_keyPurposeIDs_unfold_norm
-  (oids: list (datatype_of_asn1_type OID) {valid_keyPurposeIDs oids})
-  (x: x509_keyPurposeIDs_t oids)
+  (oids: keyPurposeIDs_oids_t)
+  // (x: x509_keyPurposeIDs_t oids)
 : Lemma (
   P.norm
     (norm_steps_x509_keyPurposeIDs "oids")
-    (serialize_x509_keyPurposeIDs_unfold_spec oids x)
+    (serialize_x509_keyPurposeIDs_unfold_spec oids)
   ==
-    (serialize_x509_keyPurposeIDs_unfold_spec oids x)
+    (serialize_x509_keyPurposeIDs_unfold_spec oids)
 )
 = P.norm_spec
     (norm_steps_x509_keyPurposeIDs "oids")
-    (serialize_x509_keyPurposeIDs_unfold_spec oids x)
+    (serialize_x509_keyPurposeIDs_unfold_spec oids)
 
 let lemma_serialize_x509_keyPurposeIDs_size_norm
-  (oids: list (datatype_of_asn1_type OID) {valid_keyPurposeIDs oids})
-  (x: x509_keyPurposeIDs_t oids)
+  (oids: keyPurposeIDs_oids_t)
+  // (x: x509_keyPurposeIDs_t oids)
 : Lemma (
   P.norm
     (norm_steps_x509_keyPurposeIDs "oids")
-    (serialize_x509_keyPurposeIDs_size_spec oids x)
+    (serialize_x509_keyPurposeIDs_size_spec oids)
   ==
-    (serialize_x509_keyPurposeIDs_size_spec oids x) /\
+    (serialize_x509_keyPurposeIDs_size_spec oids) /\
   P.norm
     (norm_steps_x509_keyPurposeIDs "oids")
-    (predicate_serialize_x509_keyPurposeIDs_size_oids oids x)
+    (predicate_serialize_x509_keyPurposeIDs_size_oids oids)
   ==
-    (predicate_serialize_x509_keyPurposeIDs_size_oids oids x)
+    (predicate_serialize_x509_keyPurposeIDs_size_oids oids)
 )
 = P.norm_spec
     (norm_steps_x509_keyPurposeIDs "oids")
-    (serialize_x509_keyPurposeIDs_size_spec oids x);
+    (serialize_x509_keyPurposeIDs_size_spec oids);
   P.norm_spec
     (norm_steps_x509_keyPurposeIDs "oids")
-    (predicate_serialize_x509_keyPurposeIDs_size_oids oids x)
+    (predicate_serialize_x509_keyPurposeIDs_size_oids oids)
 
-noextract unfold inline_for_extraction
-let oids: l: list (datatype_of_asn1_type OID) { valid_keyPurposeIDs l }
-= [@inline_let] let l = [OID_AT_CN; OID_AT_COUNTRY; OID_AT_ORGANIZATION] in
-  assert_norm (valid_keyPurposeIDs l);
-  l
+// noextract unfold inline_for_extraction
+// let oids: l: list (datatype_of_asn1_type OID) { valid_keyPurposeIDs l }
+// = [@inline_let] let l = [OID_AT_CN; OID_AT_COUNTRY; OID_AT_ORGANIZATION] in
+//   assert_norm (valid_keyPurposeIDs l);
+//   l
 
-// [@@T.postprocess_with (postprocess_x509_keyPurposeIDs (`%oids))]
-let ty = P.norm (norm_steps_x509_keyPurposeIDs (`%oids)) (x509_keyPurposeIDs_t oids)
+// // [@@T.postprocess_with (postprocess_x509_keyPurposeIDs (`%oids))]
+// let ty = P.norm (norm_steps_x509_keyPurposeIDs (`%oids)) (x509_keyPurposeIDs_t oids)
 
-let test_success
-= let tm: ty = ((OID_AT_CN, OID_AT_COUNTRY), OID_AT_ORGANIZATION) in
-()
+// let test_success
+// = let tm: ty = ((OID_AT_CN, OID_AT_COUNTRY), OID_AT_ORGANIZATION) in
+// ()
 
-(* FIXME: Why this one fails? *)
-[@expect_failure]
-let test_fail
-= let ty = P.norm (norm_steps_x509_keyPurposeIDs (`%oids)) (x509_keyPurposeIDs_t oids) in
-  let tm: ty = ((OID_AT_CN, OID_AT_COUNTRY), OID_AT_ORGANIZATION) in
-()
+// (* FIXME: Why this one fails? *)
+// [@expect_failure]
+// let test_fail
+// = let ty = P.norm (norm_steps_x509_keyPurposeIDs (`%oids)) (x509_keyPurposeIDs_t oids) in
+//   let tm: ty = ((OID_AT_CN, OID_AT_COUNTRY), OID_AT_ORGANIZATION) in
+// ()
 
 
 (* Tests
@@ -711,7 +734,7 @@ let test =
      length_of_asn1_primitive_TLV OID_AT_ORGANIZATION /\
     (serialize_x509_keyPurposeIDs_size_spec oids kpIDs)
   <= asn1_value_length_max_of_type SEQUENCE /\
- // (length_of_x509_ext_key_usage_payload_unbound oids kpIDs
+ // (length_of_x509_ext_key_usage_payload_unbounded oids kpIDs
  //  <= asn1_value_length_max_of_type OCTET_STRING) /\
  // (let _ = lemma_serialize_x509_keyPurposeIDs_size oids kpIDs;
  //          lemma_serialize_x509_ext_key_usage_payload_size_exact oids kpIDs in
@@ -737,7 +760,7 @@ let test =
 // #pop-options
 
 // let length_of_x509_ext_key_usage
-//   (oids: list (datatype_of_asn1_type OID) {valid_keyPurposeIDs oids})
+//   (oids: keyPurposeIDs_oids_t)
 //   (x: x509_ext_key_usage_payload_t oids
 //       { serialize_x509_keyPurposeIDs_size_spec oids x
 //         <= asn1_value_length_max_of_type SEQUENCE })
@@ -770,14 +793,14 @@ let test =
 
 (*)
 let parse_x509_ext_key_usage_payload
-  (oids: list (datatype_of_asn1_type OID) {valid_keyPurposeIDs oids})
+  (oids: keyPurposeIDs_oids_t)
 = parse_asn1_sequence_TLV
     (OID_EXTENDED_KEY_USAGE
      `serialize_envelop_OID_with`
      serialize_x509_keyPurposeIDs oids)
  ff
 let serialize_x509_keyPurposeIDs_sequence_TLV
-  (oids: list (datatype_of_asn1_type OID) {valid_keyPurposeIDs oids})
+  (oids: keyPurposeIDs_oids_t)
 : serializer (parse_x509_keyPurposeIDs_sequence_TLV oids)
 = serialize_asn1_sequence_TLV
     (OID_EXTENDED_KEY_USAGE_PAYLOAD
@@ -785,14 +808,14 @@ let serialize_x509_keyPurposeIDs_sequence_TLV
      serialize_x509_keyPurposeIDs oids)
 
 let lemma_serialize_x509_keyPurposeIDs_sequence_TLV_unfold
-  (oids: list (datatype_of_asn1_type OID) {valid_keyPurposeIDs oids})
+  (oids: keyPurposeIDs_oids_t)
 = lemma_serialize_asn1_sequence_TLV_unfold
     (OID_EXTENDED_KEY_USAGE_PAYLOAD
      `serialize_envelop_OID_with`
      serialize_x509_keyPurposeIDs oids)
 
 let lemma_serialize_x509_keyPurposeIDs_sequence_TLV_size
-  (oids: list (datatype_of_asn1_type OID) {valid_keyPurposeIDs oids})
+  (oids: keyPurposeIDs_oids_t)
 = lemma_serialize_asn1_sequence_TLV_size
     (OID_EXTENDED_KEY_USAGE_PAYLOAD
      `serialize_envelop_OID_with`
@@ -853,7 +876,7 @@ let x509_keyPurposeIDs_1_inbound
 = inbound_sequence_value_of (serialize_x509_keyPurposeIDs_1 oid)
 
 let x509_keyPurposeIDs_t_inbound
-  (oids: list (datatype_of_asn1_type OID) {valid_keyPurposeIDs oids})
+  (oids: keyPurposeIDs_oids_t)
 = inbound_sequence_value_of (serialize_x509_keyPurposeIDs oids)
 
 module HS = FStar.HyperStack
@@ -872,7 +895,7 @@ open FStar.Integers
 
 // #push-options "--z3rlimit 16"
 // let rec length_of_x509_keyPurposeIDs
-//   (oids: list (datatype_of_asn1_type OID) { valid_keyPurposeIDs oids})
+//   (oids: keyPurposeIDs_oids_t)
 //   (x: x509_keyPurposeIDs_t oids)
 // : GTot (l: nat {l == Seq.length (serialize (serialize_x509_keyPurposeIDs oids) x)})
 //   (decreases (List.length oids))
@@ -891,7 +914,7 @@ open FStar.Integers
 (* TODO: Check actual extraction behavior. *)
 noextract
 let rec serialize32_x509_keyPurposeIDs_backwards
-  (oids: list (datatype_of_asn1_type OID) {valid_keyPurposeIDs oids})
+  (oids: keyPurposeIDs_oids_t)
 : Tot (serializer32_backwards (serialize_x509_keyPurposeIDs oids))
   (decreases (List.length oids))
 = let oids', oid = List.Tot.Base.unsnoc oids in
@@ -904,7 +927,7 @@ let rec serialize32_x509_keyPurposeIDs_backwards
 
 noextract
 let serialize32_x509_keyPurposeIDs_sequence_TLV_backwards
-  (oids: list (datatype_of_asn1_type OID) {valid_keyPurposeIDs oids})
+  (oids: keyPurposeIDs_oids_t!)
 : serializer32_backwards (serialize_x509_keyPurposeIDs_sequence_TLV oids)
 = serialize32_asn1_sequence_TLV_backwards
   (* s32 *) (OID_EXTENDED_KEY_USAGE_PAYLOAD
