src/riot/x509/Main.fst
@@ -25,7 +25,7 @@ module B32 = FStar.Bytes
 module T = FStar.Tactics
 module P = FStar.Pervasives
 
-#set-options "--z3rlimit 32 --fuel 0 --ifuel 0"
+#set-options "--z3rlimit 32 --fuel 4 --ifuel 0"
 
 noextract unfold inline_for_extraction
 let oids: l: list (datatype_of_asn1_type OID) { valid_keyPurposeIDs l }
@@ -33,147 +33,27 @@ let oids: l: list (datatype_of_asn1_type OID) { valid_keyPurposeIDs l }
   assert_norm (valid_keyPurposeIDs l);
   l
 
-// noextract
-// let norm_kp () : Tac unit = norm [delta_only [
-//   `%x509_keyPurposeIDs_t;
-//   `%oids;
-//   `%FStar.List.Tot.Base.unsnoc;
-//   `%FStar.List.Tot.Base.splitAt;
-//   `%FStar.List.Tot.Base.length
-// ]; primops; zeta; iota]; trefl ()
-
-[@@T.postprocess_with (postprocess_x509_keyPurposeIDs (`%oids))]
-let ty = (x509_keyPurposeIDs_t oids)
-
 // [@@T.postprocess_with (postprocess_x509_keyPurposeIDs (`%oids))]
-// noextract inline_for_extraction
-// let tm: ty = get_x509_keyPurposeIDs oids
+// let ty = x509_keyPurposeIDs_t oids
 
-[@@T.postprocess_with (postprocess_x509_keyPurposeIDs (`%oids))]
-let exty = (x509_ext_key_usage_t oids)
-
-// #push-options "--fuel 4"
-// let extm: exty
-// =
-//   lemma_serialize_x509_keyPurposeIDs_size_norm oids tm;
-//   lemma_serialize_x509_keyPurposeIDs_size oids tm;
-//   x509_get_ext_extendedKeyUsage oids true
-// #pop-options
-
-let p = parse_x509_keyPurposeIDs oids
-
-let s = serialize_x509_keyPurposeIDs oids
-
-[@@T.postprocess_with (postprocess_x509_keyPurposeIDs (`%oids))]
-noextract inline_for_extraction
-let s32 = serialize32_x509_keyPurposeIDs_backwards oids
-
-[@@T.postprocess_with (postprocess_x509_keyPurposeIDs (`%oids))]
-let x =
-  let x = 1 in
-  let y = (x509_ext_key_usage_t oids) in
-  y
-
-open X509.BasicFields.Extension2
-let norm_steps_x509_keyPurposeIDs
-  (oids_name: string)
-: list P.norm_step
-= [delta_only [
-(* the parameter *)
-  oids_name;
-(* the type to extract *)
-  `%x509_keyPurposeIDs_t;
-  `%get_x509_keyPurposeIDs;
-  `%x509_ext_key_usage_payload_t;
-  `%x509_ext_key_usage_t;
-  `%x509_extension_payload_t;
-  `%x509_extension_t;
-  // `%serialize_x509_ext_key_usage_payload;
-  // `%serialize_x509_keyPurposeIDs;
-  `%inbound_sequence_value_of;
-  `%inbound_envelop_tag_with_value_of;
-  (* the Low* implementation to extract *)
-  `%serialize32_x509_keyPurposeIDs_backwards;
-  `%serialize_x509_keyPurposeIDs_size_spec;
-  `%length_of_x509_keyPurposeIDs;
-  `%len_of_x509_keyPurposeIDs;
-  `%length_of_x509_ext_key_usage;
-  `%len_of_x509_ext_key_usage_payload;
-  `%length_of_x509_ext_key_usage_payload;
-  `%len_of_x509_ext_key_usage;
-  `%length_of_x509_ext_key_usage;
-  `%x509_get_ext_extendedKeyUsage;
-(* the specs and lemmas *)
-  `%serialize_x509_keyPurposeIDs_unfold_spec;
-  `%serialize_x509_keyPurposeIDs_size_spec;
-  `%predicate_serialize_x509_keyPurposeIDs_size_oids;
-  `%lemma_serialize_x509_keyPurposeIDs_unfold;
-  `%lemma_serialize_x509_keyPurposeIDs_size;
-(* list ops *)
-  `%FStar.List.Tot.Base.unsnoc;
-  `%FStar.List.Tot.Base.splitAt;
-  `%FStar.List.Tot.Base.length;
-  `%FStar.List.Tot.Base.hd;
-(* coerce helpers *)
-  // `%coerce_parser;
-  // `%coerce_parser_serializer;
-  `%coerce_serializer32_backwards;
-  ]; primops; zeta; iota]
-
-
-let tm: ty = P.norm (norm_steps_x509_keyPurposeIDs (`%oids)) (get_x509_keyPurposeIDs oids)
+(* It works when inlining those types *)
+// [@@T.postprocess_with (postprocess_x509_keyPurposeIDs (`%oids))]
+// let exty = x509_ext_key_usage_t oids
 
 #push-options "--fuel 4"
 [@@T.postprocess_with (postprocess_x509_keyPurposeIDs (`%oids))]
-let xx =
-  // let tm: ty = P.norm (norm_steps_x509_keyPurposeIDs (`%oids)) (get_x509_keyPurposeIDs oids) in
-  lemma_serialize_x509_keyPurposeIDs_size_norm oids tm;
-  lemma_serialize_x509_keyPurposeIDs_size oids tm;
-  assert (
-    serialize_x509_keyPurposeIDs_size_spec oids tm <=
-    asn1_value_length_max_of_type (SEQUENCE) /\
-    length_of_x509_ext_key_usage_payload_unbound oids tm <=
-    asn1_value_length_max_of_type (OCTET_STRING) /\
-    length_of_opaque_serialization (serialize_x509_keyPurposeIDs oids) tm
-    <= asn1_value_length_max_of_type SEQUENCE
-  );
-  // lemma_serialize_x509_ext_key_usage_payload_size_exact oids tm;
-  len_of_x509_ext_key_usage_payload oids tm
-
-let f ()
-= let extm: exty = (x509_get_ext_extendedKeyUsage oids true) in
-  1
-
-// #push-options "--fuel 4"
 let main ()
 : HST.ST C.exit_code
   (requires fun h -> True)
   (ensures fun _ _ _ -> True)
 =
-  // HST.push_frame ();
-  // let b = B.alloca 0uy 100ul in
-  // let tm: ty = ((OID_AT_CN, OID_AT_COUNTRY), OID_AT_ORGANIZATION) in
-  let tm: ty = P.norm (norm_steps_x509_keyPurposeIDs (`%oids)) (get_x509_keyPurposeIDs oids) in
-  lemma_serialize_x509_keyPurposeIDs_size_norm oids tm;
-  lemma_serialize_x509_keyPurposeIDs_size oids tm;
-  assert (
-    serialize_x509_keyPurposeIDs_size_spec oids tm <=
-    asn1_value_length_max_of_type (SEQUENCE) /\
-    length_of_x509_ext_key_usage_payload_unbound oids tm <=
-    asn1_value_length_max_of_type (OCTET_STRING) /\
-    length_of_opaque_serialization (serialize_x509_keyPurposeIDs oids) tm
-    <= asn1_value_length_max_of_type SEQUENCE /\
-   (let _ = lemma_serialize_x509_ext_key_usage_payload_size_exact oids tm in
-    X509.BasicFields.Extension2.length_of_x509_extension_payload_unbounded
-      (OID_EXTENDED_KEY_USAGE)
-      (serialize_x509_ext_key_usage_payload oids)
-      (tm)
-      (P.norm (norm_steps_x509_keyPurposeIDs (`%oids)) length_of_x509_ext_key_usage_payload oids tm)
-    <= asn1_value_length_max_of_type (SEQUENCE))
-  );
-  let extm: exty = P.norm_spec (norm_steps_x509_keyPurposeIDs (`%oids)) (x509_get_ext_extendedKeyUsage oids true);
-                   P.norm      (norm_steps_x509_keyPurposeIDs (`%oids)) (x509_get_ext_extendedKeyUsage oids true) in
-  // let tm2: ty = snd extm in
-  // let r = s32 tm b 50ul in
-  // HST.pop_frame ();
+  HST.push_frame ();
+  let b = B.alloca 0uy 100ul in
+  let tm: x509_keyPurposeIDs_t oids = get_x509_keyPurposeIDs oids in
+  (* Prf *) lemma_serialize_x509_keyPurposeIDs_size oids tm;
+  let extm: x509_ext_key_usage_t oids = x509_get_ext_extendedKeyUsage oids true in
+  (* Prf *) lemma_serialize_x509_ext_key_usage_size_exact oids extm;
+  let r = serialize32_x509_keyPurposeIDs_backwards oids tm b 50ul in
+  let r = serialize32_x509_ext_key_usage_backwards oids extm b 50ul in
+  HST.pop_frame ();
   C.EXIT_SUCCESS
