src/riot/x509/X509.ExtFields.ExtendedKeyUsage.Tests.fst
@@ -1,5 +1,5 @@
 module X509.ExtFields.ExtendedKeyUsage.Tests
-
+(*)
 open LowParse.Spec.Base
 open LowParse.Spec.Combinators
 
@@ -34,22 +34,6 @@ let oids: l: list (datatype_of_asn1_type OID) { valid_keyPurposeIDs l }
 //   `%FStar.List.Tot.Base.hd;
 // ]; primops; zeta; iota]; trefl ()
 
-(*)
-#push-options "--fuel 0 --ifuel 0"
-// [@@T.postprocess_with (postprocess_x509_keyPurposeIDs (`%oids))]
-let ty = P.norm      (norm_steps_x509_keyPurposeIDs (`%oids)) (x509_keyPurposeIDs_t oids)
-
-[@expect_failure]
-let test_fail
-= let ty = P.norm      (norm_steps_x509_keyPurposeIDs (`%oids)) (x509_keyPurposeIDs_t oids) in
-  let tm: ty = ((OID_AT_CN, OID_AT_COUNTRY), OID_AT_ORGANIZATION) in
-()
-
-let test_success
-= //let ty = P.norm      (norm_steps_x509_keyPurposeIDs (`%oids)) (x509_keyPurposeIDs_t oids) in
-  let tm: ty = ((OID_AT_CN, OID_AT_COUNTRY), OID_AT_ORGANIZATION) in
-()
-
 let tm: ty = ((OID_AT_CN, OID_AT_COUNTRY), OID_AT_ORGANIZATION)
 
 let p = parse_x509_keyPurposeIDs oids
@@ -69,22 +53,21 @@ let lemma_serialize_x509_keyPurposeIDs_unfold_test ()
   lemma_serialize_x509_keyPurposeIDs_unfold_norm oids tm;
   lemma_serialize_x509_keyPurposeIDs_unfold oids tm
 
-#push-options "--z3rlimit 32 --fuel 0 --ifuel 0"
+#push-options "--z3rlimit 32 --fuel 4 --ifuel 0"
 // [@@T.postprocess_with (postprocess_x509_keyPurposeIDs (`%oids))]
-[@expect_failure]
 let lemma_serialize_x509_keyPurposeIDs_size_test ()
 : Lemma (
   // let ty = P.norm_spec (norm_steps_x509_keyPurposeIDs (`%oids)) (x509_keyPurposeIDs_t oids);
   //          P.norm      (norm_steps_x509_keyPurposeIDs (`%oids)) (x509_keyPurposeIDs_t oids) in
-  let tm: ty = ((OID_AT_CN, OID_AT_COUNTRY), OID_AT_ORGANIZATION) in
+  // let tm: ty = ((OID_AT_CN, OID_AT_COUNTRY), OID_AT_ORGANIZATION) in
  // length_of_opaque_serialization s tm < 100
  serialize_x509_keyPurposeIDs_size_spec oids tm < 100
 )
-= admit();
-  let ty = (x509_keyPurposeIDs_t oids) in
-  let tm: ty = ((OID_AT_CN, OID_AT_COUNTRY), OID_AT_ORGANIZATION) in
+= //admit();
+  // let ty = (x509_keyPurposeIDs_t oids) in
+  // let tm: ty = ((OID_AT_CN, OID_AT_COUNTRY), OID_AT_ORGANIZATION) in
   //P.norm_spec (norm_steps_x509_keyPurposeIDs (`%oids)) (serialize_x509_keyPurposeIDs_unfold_spec oids tm);
-  lemma_serialize_x509_keyPurposeIDs_size_norm oids tm;
+  // lemma_serialize_x509_keyPurposeIDs_size_norm oids tm;
   lemma_serialize_x509_keyPurposeIDs_size oids tm
   // lemma_serialize_asn1_oid_TLV_of_size OID_AT_CN OID_AT_CN;
   // lemma_serialize_asn1_oid_TLV_of_size OID_AT_COUNTRY OID_AT_COUNTRY;
